veric/SeparationLogicSoundness.v
@@ -40,8 +40,8 @@ Axiom semax_prog_rule :
      Genv.init_mem prog = Some m ->
      { b : block & { q : corestate &
        (Genv.find_symbol (globalenv prog) (prog_main prog) = Some b) *
-       (forall jm, m_dry jm = m -> semantics.initial_core (juicy_core_sem cl_core_sem) h
-                    (globalenv prog) jm (Vptr b Ptrofs.zero) nil = Some (q, None)) *
+       (forall jm, m_dry jm = m -> core_semantics.initial_core (juicy_core_sem (cl_core_sem (globalenv prog))) h
+                    jm q (Vptr b Ptrofs.zero) nil) *
        forall n, { jm |
        m_dry jm = m /\ level jm = n /\
        (forall z, jsafeN (@OK_spec Espec) (globalenv prog) n z q jm) /\
