veric/semax_congruence.v
@@ -34,13 +34,13 @@ Section extensions.
 Context (Espec : OracleKind).
 
 Lemma safeN_step_jsem_spec: forall gx vx tx n k ora jm,
-  @jsafeN_ _ _ _ (fun x => Genv.genv_symb (genv_genv x)) (cl_core_sem) OK_spec
+  @jsafeN_ _ _ _ (fun x => Genv.genv_symb (genv_genv x)) (cl_core_sem gx) OK_spec
     gx (S n) ora (State vx tx k) jm <->
   exists c' m', (cl_step gx (State vx tx k) (m_dry jm) c' (m_dry m') /\
   resource_decay (nextblock (m_dry jm)) (m_phi jm) (m_phi m') /\
   level jm = S (level m') /\
   ghost_of (m_phi m') = ghost_approx m' (ghost_of (m_phi jm)) /\
-  jm_bupd (@jsafeN_ _ _ _ (fun x => Genv.genv_symb (genv_genv x)) (cl_core_sem) OK_spec gx n ora c') m').
+  jm_bupd (@jsafeN_ _ _ _ (fun x => Genv.genv_symb (genv_genv x)) (cl_core_sem gx) OK_spec gx n ora c') m').
 Proof.
   intros.
   split; intros.
